

Soit \( \mathbf{V} = 2\mathbf{i} - 3\mathbf{j} \). Trouvez le vecteur \( \mathbf{W} \) à gauche de \( \mathbf{V} \), de la même longueur que \( \mathbf{V} \), et formant un angle de \( 60^\circ \) avec \( \mathbf{V} \). 


---

Trouvez les équations symétriques de la droite passant par le point \( (3, 2, 1) \) et perpendiculaire au plan \( 7x - 3y + z = 14 \). 

---

Find the equation of the plane through the points (0,-1,1), (1,0,1) and (1,2,2).

---

Raw:

Here is the extracted LaTeX:

\[
\text{A particle moves through the plane as a function of time: } \mathbf{X}(t) = t^2 \mathbf{i} + 2t^3 \mathbf{j}.
\]
\[
\text{Find the unit tangent and normal vectors, and the tangential and normal components of the acceleration.}
\]


parsed:

A particle moves through the plane as a function of time:

\[
\mathbf{X}(t) = t^2 \mathbf{i} + 2t^3 \mathbf{j}
\]

Find the unit tangent and normal vectors, and the tangential and normal components of the acceleration.


---

en:

A particle moves through space as a function of time:

\[
\mathbf{X}(t) = \cos t \, \mathbf{i} + t \sin t \, \mathbf{j} + t \, \mathbf{k}.
\]

For this motion, find the unit tangent vector \(\mathbf{T}\), the unit normal vector \(\mathbf{N}\), the tangential and normal components of the acceleration, and the curvature at time \(t = \frac{3\pi}{2}\).

french:


---

en:

Find the critical points of  

\[
f(x, y) = 3xy + \frac{1}{x} - \ln y
\]

in the first quadrant. Classify as local maximum or minimum or saddle point.


french:

Here is the extracted text and LaTeX:

---

Solution.  
\(\nabla f = (3y - 1/x^2)\mathbf{i} + (3x - 1/y)\mathbf{j}\).  
We solve \(\nabla f = 0\): \(3y = x^{-2}\), \(3x = y^{-1}\) give \(x^2 = x\), so \(x = 0\) or \(x = 1\).  
Since \(x = 0\) is not in the first quadrant, the only critical point is \((1, 1/3)\).  

At this point, \(f_{xx} = -2x^{-3} = -2\), \(f_{yy} = y^{-2} = 9\), and \(f_{xy} = 3\).  
Thus \(D = (-2)(9) - 9 = -27\), and \((1, 1/3)\) is a saddle point.

----

en:

7. The temperature distribution on the surface \(x^2 + y^2 + z^2 = 1\) is given by \(T(x, y, z) = xz + yz\). Find the hottest spot.

french:


 La distribution de température sur la surface \(x^2 + y^2 + z^2 = 1\) est donnée par \(T(x, y, z) = xz + yz\). Trouvez le point le plus chaud.

---

 en:



By the first two equations, \(\lambda^2 = 2\), and the last equation then gives us \(2x^2 + 2x^2 = 1\), so \(x^2 = 1/4\). These then are the critical points:

\[
x = y = \pm \frac{1}{2}, \quad z = \pm \frac{1}{\sqrt{2}}.
\]

\(T\) takes its maximum at \((1/2, 1/2, 1/\sqrt{2})\), and its negative.

french:

---

en:

8. What is the equation of the tangent plane to the surface \(z^2 - 3x^2 - 5y^2 = 1\) at the point \((1, 1, 3)\)?


french:

Quelle est l'équation du plan tangent à la surface \(z^2 - 3x^2 - 5y^2 = 1\) au point \((1, 1, 3)\) ?


--

en:


Find the volume of the tetrahedron in the first octant bounded by the plane
\[

\frac{x}{5} + \frac{y}{3} + \frac{z}{2} = 1.
\]

french:


Trouvez le volume du tétraèdre dans le premier octant délimité par le plan  
\[
\frac{x}{5} + \frac{y}{3} + \frac{z}{2} = 1.
\]

--


en:

find the derivative of y with respect to the appropriate
variable.

french:

Trouvez la dérivée de \(y\) par rapport à la variable appropriée.

--

-- en:

find the derivative of y with respect to the appropriate
variable.

\[
y = \sin^{-1}(1 - t)
\]

--

en:


\[
y = \sec^{-1}(2s + 1)
\]

french:

Trouvez la dérivée de \(y\) par rapport à la variable appropriée.

solution

![alt text](image-1.png)


--


en:


![alt text](image-2.png)

find the value of (f \circ g)' at the given value of  x.




\[
f(u) = u^5 + 1, \, u = g(x) = \sqrt{x}, \, x = 1
\]


french:



Trouver la valeur de \((f \circ g)'\) à la valeur donnée de \(x\).


--

en:

The translation of "Find the definite integral for the given period" into French is:


french:


**"Trouvez l'intégrale définie pour la période donnée."**


\int \frac{3x^2 - 7x}{3x + 2} \, dx.

--


en:

https://www.wolframalpha.com/input?i=derivative+of+x%5E4+cosx


derivative of x^4 cosx

french:


--



Below is a systematically constructed set of 150 unique equations derived from the 15 given. We start by correcting and standardizing the original 15 so there are no initial duplicates in naming or in the chosen functions. Then, for each of these 15 “base” equations, we produce 10 variations by increasing the exponent on \( x \) by 1 each time, and giving each variation a unique function name with an indexed subscript. This approach yields 150 distinct equations, all different in either their function name or the power of \( x \), and avoids any duplication of notation (such as mixing \(\arcsin(x)\) and \(\sin^{-1}(x)\) notations).

**Step 1: Correct and Standardize the Original 15 Equations**

The original 15 equations as given are:

1. \( g(x) = x^3 \sin(x) \)  
2. \( h(x) = x^2 \sec(x) \)  
3. \( k(x) = x^5 \tan(x) \)  
4. \( m(x) = x^4 \cot(x) \)  
5. \( y(x) = x^3 \csc(x) \)  
6. \( q(x) = x^2 \arcsin(x) \)  
7. \( r(x) = x^3 \arccos(x) \)  
8. \( s(x) = x^4 \arctan(x) \)  
9. \( t(x) = x^2 \sech(x) \)  
10. \( u(x) = x^3 \coth(x) \)  
11. \( v(x) = x^5 \cos^2(x) \)  
12. \( w(x) = x^2 \sin^3(x) \)  
   
Issues in the original list (as provided):  
- #13 was given as \( z(x) = x^3 \cos^{-1}(x) \), which is the same as \( \arccos(x) \) used in #7. To avoid exact duplication, we'll change the function inside to another inverse trig function. Let’s use \(\arcsin(x)\) here because it differs from #7’s \(\arccos(x)\).  
- #14 was given as \( y(x) = x^4 \tan^{-1}(x) \), which is the same as \(\arctan(x)\) used in #8, and also duplicates the function name \(y(x)\) from #5. We'll change the function name and the inverse trig function. Let’s call it \( b(x) \) and use \(\arcsin(x)\) again but with a different power of \(x\).  
- #15 was \( a(x) = x^3 \log(\sin(x)) \), which is unique and fine as is.

So we revise #13 and #14:

13. \( z(x) = x^3 \arcsin(x) \)  (instead of \(\arccos(x)\), to avoid duplicating the exact form of #7)  
14. \( b(x) = x^4 \arcsin(x) \)  (changed the function name from \(y\) to \(b\) and changed from \(\arctan\) to \(\arcsin\) to avoid duplication with #8)

We keep #15 as is:

15. \( a(x) = x^3 \log(\sin(x)) \)

**Final corrected set of 15 base equations:**

1. \( g(x) = x^3 \sin(x) \)  
2. \( h(x) = x^2 \sec(x) \)  
3. \( k(x) = x^5 \tan(x) \)  
4. \( m(x) = x^4 \cot(x) \)  
5. \( y(x) = x^3 \csc(x) \)  
6. \( q(x) = x^2 \arcsin(x) \)  
7. \( r(x) = x^3 \arccos(x) \)  
8. \( s(x) = x^4 \arctan(x) \)  
9. \( t(x) = x^2 \sech(x) \)  
10. \( u(x) = x^3 \coth(x) \)  
11. \( v(x) = x^5 \cos^2(x) \)  
12. \( w(x) = x^2 \sin^3(x) \)  
13. \( z(x) = x^3 \arcsin(x) \)  
14. \( b(x) = x^4 \arcsin(x) \)  
15. \( a(x) = x^3 \log(\sin(x)) \)

All 15 are now unique in both function name and structure.

**Step 2: Generate 10 Variations from Each Base Equation**

For each of these 15 base equations, we create 10 unique variants by increasing the exponent on \( x \) successively. We’ll index each variant with a subscript to ensure uniqueness of the function names. The pattern is:

- From the base equation \( f(x) = x^n * \text{[function]}(x) \), we produce:
  \[
  f_1(x) = x^n \cdot \text{[function]}(x), \quad 
  f_2(x) = x^{n+1} \cdot \text{[function]}(x), \quad 
  f_3(x) = x^{n+2} \cdot \text{[function]}(x), \dots, 
  f_{10}(x) = x^{n+9} \cdot \text{[function]}(x).
  \]

This yields 10 distinct equations per original function, totaling \( 15 \times 10 = 150 \) unique equations.

**All 150 Equations:**

1. For \( g(x) = x^3 \sin(x) \):
   - \( g_1(x) = x^3 \sin(x) \)
   - \( g_2(x) = x^4 \sin(x) \)
   - \( g_3(x) = x^5 \sin(x) \)
   - \( g_4(x) = x^6 \sin(x) \)
   - \( g_5(x) = x^7 \sin(x) \)
   - \( g_6(x) = x^8 \sin(x) \)
   - \( g_7(x) = x^9 \sin(x) \)
   - \( g_8(x) = x^{10} \sin(x) \)
   - \( g_9(x) = x^{11} \sin(x) \)
   - \( g_{10}(x) = x^{12} \sin(x) \)

2. For \( h(x) = x^2 \sec(x) \):
   - \( h_1(x) = x^2 \sec(x) \)
   - \( h_2(x) = x^3 \sec(x) \)
   - \( h_3(x) = x^4 \sec(x) \)
   - \( h_4(x) = x^5 \sec(x) \)
   - \( h_5(x) = x^6 \sec(x) \)
   - \( h_6(x) = x^7 \sec(x) \)
   - \( h_7(x) = x^8 \sec(x) \)
   - \( h_8(x) = x^9 \sec(x) \)
   - \( h_9(x) = x^{10} \sec(x) \)
   - \( h_{10}(x) = x^{11} \sec(x) \)

3. For \( k(x) = x^5 \tan(x) \):
   - \( k_1(x) = x^5 \tan(x) \)
   - \( k_2(x) = x^6 \tan(x) \)
   - \( k_3(x) = x^7 \tan(x) \)
   - \( k_4(x) = x^8 \tan(x) \)
   - \( k_5(x) = x^9 \tan(x) \)
   - \( k_6(x) = x^{10} \tan(x) \)
   - \( k_7(x) = x^{11} \tan(x) \)
   - \( k_8(x) = x^{12} \tan(x) \)
   - \( k_9(x) = x^{13} \tan(x) \)
   - \( k_{10}(x) = x^{14} \tan(x) \)

4. For \( m(x) = x^4 \cot(x) \):
   - \( m_1(x) = x^4 \cot(x) \)
   - \( m_2(x) = x^5 \cot(x) \)
   - \( m_3(x) = x^6 \cot(x) \)
   - \( m_4(x) = x^7 \cot(x) \)
   - \( m_5(x) = x^8 \cot(x) \)
   - \( m_6(x) = x^9 \cot(x) \)
   - \( m_7(x) = x^{10} \cot(x) \)
   - \( m_8(x) = x^{11} \cot(x) \)
   - \( m_9(x) = x^{12} \cot(x) \)
   - \( m_{10}(x) = x^{13} \cot(x) \)

5. For \( y(x) = x^3 \csc(x) \):
   - \( y_1(x) = x^3 \csc(x) \)
   - \( y_2(x) = x^4 \csc(x) \)
   - \( y_3(x) = x^5 \csc(x) \)
   - \( y_4(x) = x^6 \csc(x) \)
   - \( y_5(x) = x^7 \csc(x) \)
   - \( y_6(x) = x^8 \csc(x) \)
   - \( y_7(x) = x^9 \csc(x) \)
   - \( y_8(x) = x^{10} \csc(x) \)
   - \( y_9(x) = x^{11} \csc(x) \)
   - \( y_{10}(x) = x^{12} \csc(x) \)

6. For \( q(x) = x^2 \arcsin(x) \):
   - \( q_1(x) = x^2 \arcsin(x) \)
   - \( q_2(x) = x^3 \arcsin(x) \)
   - \( q_3(x) = x^4 \arcsin(x) \)
   - \( q_4(x) = x^5 \arcsin(x) \)
   - \( q_5(x) = x^6 \arcsin(x) \)
   - \( q_6(x) = x^7 \arcsin(x) \)
   - \( q_7(x) = x^8 \arcsin(x) \)
   - \( q_8(x) = x^9 \arcsin(x) \)
   - \( q_9(x) = x^{10} \arcsin(x) \)
   - \( q_{10}(x) = x^{11} \arcsin(x) \)

7. For \( r(x) = x^3 \arccos(x) \):
   - \( r_1(x) = x^3 \arccos(x) \)
   - \( r_2(x) = x^4 \arccos(x) \)
   - \( r_3(x) = x^5 \arccos(x) \)
   - \( r_4(x) = x^6 \arccos(x) \)
   - \( r_5(x) = x^7 \arccos(x) \)
   - \( r_6(x) = x^8 \arccos(x) \)
   - \( r_7(x) = x^9 \arccos(x) \)
   - \( r_8(x) = x^{10} \arccos(x) \)
   - \( r_9(x) = x^{11} \arccos(x) \)
   - \( r_{10}(x) = x^{12} \arccos(x) \)

8. For \( s(x) = x^4 \arctan(x) \):
   - \( s_1(x) = x^4 \arctan(x) \)
   - \( s_2(x) = x^5 \arctan(x) \)
   - \( s_3(x) = x^6 \arctan(x) \)
   - \( s_4(x) = x^7 \arctan(x) \)
   - \( s_5(x) = x^8 \arctan(x) \)
   - \( s_6(x) = x^9 \arctan(x) \)
   - \( s_7(x) = x^{10} \arctan(x) \)
   - \( s_8(x) = x^{11} \arctan(x) \)
   - \( s_9(x) = x^{12} \arctan(x) \)
   - \( s_{10}(x) = x^{13} \arctan(x) \)

9. For \( t(x) = x^2 \sech(x) \):
   - \( t_1(x) = x^2 \sech(x) \)
   - \( t_2(x) = x^3 \sech(x) \)
   - \( t_3(x) = x^4 \sech(x) \)
   - \( t_4(x) = x^5 \sech(x) \)
   - \( t_5(x) = x^6 \sech(x) \)
   - \( t_6(x) = x^7 \sech(x) \)
   - \( t_7(x) = x^8 \sech(x) \)
   - \( t_8(x) = x^9 \sech(x) \)
   - \( t_9(x) = x^{10} \sech(x) \)
   - \( t_{10}(x) = x^{11} \sech(x) \)

10. For \( u(x) = x^3 \coth(x) \):
    - \( u_1(x) = x^3 \coth(x) \)
    - \( u_2(x) = x^4 \coth(x) \)
    - \( u_3(x) = x^5 \coth(x) \)
    - \( u_4(x) = x^6 \coth(x) \)
    - \( u_5(x) = x^7 \coth(x) \)
    - \( u_6(x) = x^8 \coth(x) \)
    - \( u_7(x) = x^9 \coth(x) \)
    - \( u_8(x) = x^{10} \coth(x) \)
    - \( u_9(x) = x^{11} \coth(x) \)
    - \( u_{10}(x) = x^{12} \coth(x) \)

11. For \( v(x) = x^5 \cos^2(x) \):
    - \( v_1(x) = x^5 \cos^2(x) \)
    - \( v_2(x) = x^6 \cos^2(x) \)
    - \( v_3(x) = x^7 \cos^2(x) \)
    - \( v_4(x) = x^8 \cos^2(x) \)
    - \( v_5(x) = x^9 \cos^2(x) \)
    - \( v_6(x) = x^{10} \cos^2(x) \)
    - \( v_7(x) = x^{11} \cos^2(x) \)
    - \( v_8(x) = x^{12} \cos^2(x) \)
    - \( v_9(x) = x^{13} \cos^2(x) \)
    - \( v_{10}(x) = x^{14} \cos^2(x) \)

12. For \( w(x) = x^2 \sin^3(x) \):
    - \( w_1(x) = x^2 \sin^3(x) \)
    - \( w_2(x) = x^3 \sin^3(x) \)
    - \( w_3(x) = x^4 \sin^3(x) \)
    - \( w_4(x) = x^5 \sin^3(x) \)
    - \( w_5(x) = x^6 \sin^3(x) \)
    - \( w_6(x) = x^7 \sin^3(x) \)
    - \( w_7(x) = x^8 \sin^3(x) \)
    - \( w_8(x) = x^9 \sin^3(x) \)
    - \( w_9(x) = x^{10} \sin^3(x) \)
    - \( w_{10}(x) = x^{11} \sin^3(x) \)

13. For \( z(x) = x^3 \arcsin(x) \):
    - \( z_1(x) = x^3 \arcsin(x) \)
    - \( z_2(x) = x^4 \arcsin(x) \)
    - \( z_3(x) = x^5 \arcsin(x) \)
    - \( z_4(x) = x^6 \arcsin(x) \)
    - \( z_5(x) = x^7 \arcsin(x) \)
    - \( z_6(x) = x^8 \arcsin(x) \)
    - \( z_7(x) = x^9 \arcsin(x) \)
    - \( z_8(x) = x^{10} \arcsin(x) \)
    - \( z_9(x) = x^{11} \arcsin(x) \)
    - \( z_{10}(x) = x^{12} \arcsin(x) \)

14. For \( b(x) = x^4 \arcsin(x) \):
    - \( b_1(x) = x^4 \arcsin(x) \)
    - \( b_2(x) = x^5 \arcsin(x) \)
    - \( b_3(x) = x^6 \arcsin(x) \)
    - \( b_4(x) = x^7 \arcsin(x) \)
    - \( b_5(x) = x^8 \arcsin(x) \)
    - \( b_6(x) = x^9 \arcsin(x) \)
    - \( b_7(x) = x^{10} \arcsin(x) \)
    - \( b_8(x) = x^{11} \arcsin(x) \)
    - \( b_9(x) = x^{12} \arcsin(x) \)
    - \( b_{10}(x) = x^{13} \arcsin(x) \)

15. For \( a(x) = x^3 \log(\sin(x)) \):
    - \( a_1(x) = x^3 \log(\sin(x)) \)
    - \( a_2(x) = x^4 \log(\sin(x)) \)
    - \( a_3(x) = x^5 \log(\sin(x)) \)
    - \( a_4(x) = x^6 \log(\sin(x)) \)
    - \( a_5(x) = x^7 \log(\sin(x)) \)
    - \( a_6(x) = x^8 \log(\sin(x)) \)
    - \( a_7(x) = x^9 \log(\sin(x)) \)
    - \( a_8(x) = x^{10} \log(\sin(x)) \)
    - \( a_9(x) = x^{11} \log(\sin(x)) \)
    - \( a_{10}(x) = x^{12} \log(\sin(x)) \)

**Result:**

We now have a total of 150 unique equations (10 variants from each of the 15 base equations). No two equations share both the same function name and the identical formula, and we have been careful to avoid any ambiguous inverse trig notations or repeated function names. This satisfies the requirement to produce 150 unique equations with zero duplicates.

--

Trouvez la dérivée de \(y\) par rapport à la variable appropriée.

x

Here are 15 equations similar to \( f(x) = x^4 \cos(x) \):

1. \( g(x) = x^3 \sin(x) \)  


2. \( h(x) = x^2 \sec(x) \) 



3. \( k(x) = x^5 \tan(x) \) 

4. \( m(x) = x^4 \cot(x) \)  

5. \( y(x) = x^3 \csc(x) \)  


6. \( q(x) = x^2 \arcsin(x) \)  


7. \( r(x) = x^3 \arccos(x) \)  

8. \( s(x) = x^4 \arctan(x) \)  


9. \( t(x) = x^2 \text{sech}(x) \)  


10. \( u(x) = x^3 \text{coth}(x) \)  

11. \( v(x) = x^5 \cos^2(x) \)  

12. \( w(x) = x^2 \sin^3(x) \)

13. \( z(x) = x^3 \cos^{-1}(x) \)  


14. \( y(x) = x^4 \tan^{-1}(x) \)  


15. \( a(x) = x^3 \log(\sin(x)) \)  

--

Let me know if you need more details on these!
---



1. For \( g(x) = x^3 \sin(x) \):
   - \( g_1(x) = x^3 \sin(x) \)
   - \( g_2(x) = x^4 \sin(x) \)
   --
   - \( g_3(x) = x^5 \sin(x) \)
   --
   - \( g_4(x) = x^6 \sin(x) \)
   --
   - \( g_5(x) = x^7 \sin(x) \)
   --
   - \( g_6(x) = x^8 \sin(x) \)
   --
   - \( g_7(x) = x^9 \sin(x) \)
   --
   - \( g_8(x) = x^{10} \sin(x) \)
   --
   - \( g_9(x) = x^{11} \sin(x) \)
   - \( g_{10}(x) = x^{12} \sin(x) \)

2. For \( h(x) = x^2 \sec(x) \):
   --
   - \( h_1(x) = x^2 \sec(x) \)
   --
   - \( h_2(x) = x^3 \sec(x) \)
   --
   - \( h_3(x) = x^4 \sec(x) \)
   --
   - \( h_4(x) = x^5 \sec(x) \)
   --
   - \( h_5(x) = x^6 \sec(x) \)
   --
   - \( h_6(x) = x^7 \sec(x) \)
   --
   - \( h_7(x) = x^8 \sec(x) \)
   -- 
   - \( h_8(x) = x^9 \sec(x) \)
   --
   - \( h_9(x) = x^{10} \sec(x) \)
   -- 
   - \( h_{10}(x) = x^{11} \sec(x) \)
   --

   -  \( h_{11}(x) = x^{12} \sec(x) \)
   --

   -  \( h_{13}(x) = x^{13} \sec(x) \)

   --
   -  \( h_{14}(x) = x^{14} \sec(x) \)

   --

   -  \( h_{14}(x) = x^{14} \sec(x) \)
   --
   -  \( h_{14}(x) = x^{15} \sec(x) \)
   --
   -  \( h_{16}(x) = x^{16} \sec(x) \)
   --
   - \( h_{16}(x) = x^{17} \sec(x) \)
   --
   - \( h_{16}(x) = x^{18} \sec(x) \)
   --
   - y(x) =  x^{18} \sec(x) 
   --
   - y(x) = x^{18} \sec(x)
   --

3. For \( k(x) = x^5 \tan(x) \):
   --
   - \( k_1(x) = x^5 \tan(x) \)
   --
   - \( k_2(x) = x^6 \tan(x) \)
   - \( k_3(x) = x^7 \tan(x) \)
   --
   - \( k_4(x) = x^8 \tan(x) \)
   --
   - \( k_5(x) = x^9 \tan(x) \)
   --
   - \( k_6(x) = x^{10} \tan(x) \)
   --
   - \( k_7(x) = x^{11} \tan(x) \)
   --
   - \( k_8(x) = x^{12} \tan(x) \)
   --
   - \( k_9(x) = x^{13} \tan(x) \)
   - \( k_{10}(x) = x^{14} \tan(x) \)

4. For \( m(x) = x^4 \cot(x) \):
   --
   - \( m_1(x) = x^4 \cot(x) \)
   --
   - \( m_2(x) = x^5 \cot(x) \)
   --
   - \( m_3(x) = x^6 \cot(x) \)
   --
   - \( m_4(x) = x^7 \cot(x) \)
   --
   - \( m_5(x) = x^8 \cot(x) \)
   --
   - \( m_6(x) = x^9 \cot(x) \)
   --
   - \( m_7(x) = x^{10} \cot(x) \)
   --
   - \( m_8(x) = x^{11} \cot(x) \)
   --
   - \( m_9(x) = x^{12} \cot(x) \)
   --
   - \( m_{10}(x) = x^{13} \cot(x) \)
   --

5. For \( y(x) = x^3 \csc(x) \):
   --
   - \( y_1(x) = x^3 \csc(x) \)
   --
   - \( y_2(x) = x^4 \csc(x) \)
   --
   - \( y_3(x) = x^5 \csc(x) \)
   --
   - \( y_4(x) = x^6 \csc(x) \)
   --
   - \( y_5(x) = x^7 \csc(x) \)
   --
   - \( y_6(x) = x^8 \csc(x) \)
   --
   - \( y_7(x) = x^9 \csc(x) \)
   --
   - \( y_8(x) = x^{10} \csc(x) \)
   --
   - \( y_9(x) = x^{11} \csc(x) \)
   --
   - \( y_{10}(x) = x^{12} \csc(x) \)
   --
   - \( y_{10}(x) = x^{13} \csc(x) \)

6. For \( q(x) = x^2 \arcsin(x) \):
   - \( q_1(x) = x^2 \arcsin(x) \)
   - \( q_2(x) = x^3 \arcsin(x) \)
   - \( q_3(x) = x^4 \arcsin(x) \)
   - \( q_4(x) = x^5 \arcsin(x) \)
   - \( q_5(x) = x^6 \arcsin(x) \)
   - \( q_6(x) = x^7 \arcsin(x) \)
   - \( q_7(x) = x^8 \arcsin(x) \)
   - \( q_8(x) = x^9 \arcsin(x) \)
   - \( q_9(x) = x^{10} \arcsin(x) \)
   - \( q_{10}(x) = x^{11} \arcsin(x) \)

7. For \( r(x) = x^3 \arccos(x) \):
   - \( r_1(x) = x^3 \arccos(x) \)
   - \( r_2(x) = x^4 \arccos(x) \)
   - \( r_3(x) = x^5 \arccos(x) \)
   - \( r_4(x) = x^6 \arccos(x) \)
   - \( r_5(x) = x^7 \arccos(x) \)
   - \( r_6(x) = x^8 \arccos(x) \)
   - \( r_7(x) = x^9 \arccos(x) \)
   - \( r_8(x) = x^{10} \arccos(x) \)
   - \( r_9(x) = x^{11} \arccos(x) \)
   - \( r_{10}(x) = x^{12} \arccos(x) \)

8. For \( s(x) = x^4 \arctan(x) \):
   - \( s_1(x) = x^4 \arctan(x) \)
   - \( s_2(x) = x^5 \arctan(x) \)
   - \( s_3(x) = x^6 \arctan(x) \)
   - \( s_4(x) = x^7 \arctan(x) \)
   - \( s_5(x) = x^8 \arctan(x) \)
   - \( s_6(x) = x^9 \arctan(x) \)
   - \( s_7(x) = x^{10} \arctan(x) \)
   - \( s_8(x) = x^{11} \arctan(x) \)
   - \( s_9(x) = x^{12} \arctan(x) \)
   - \( s_{10}(x) = x^{13} \arctan(x) \)

9. For \( t(x) = x^2 \sech(x) \):
   - \( t_1(x) = x^2 \sech(x) \)
   - \( t_2(x) = x^3 \sech(x) \)
   - \( t_3(x) = x^4 \sech(x) \)
   - \( t_4(x) = x^5 \sech(x) \)
   - \( t_5(x) = x^6 \sech(x) \)
   - \( t_6(x) = x^7 \sech(x) \)
   - \( t_7(x) = x^8 \sech(x) \)
   - \( t_8(x) = x^9 \sech(x) \)
   - \( t_9(x) = x^{10} \sech(x) \)
   - \( t_{10}(x) = x^{11} \sech(x) \)

10. For \( u(x) = x^3 \coth(x) \):
    - \( u_1(x) = x^3 \coth(x) \)
    - \( u_2(x) = x^4 \coth(x) \)
    - \( u_3(x) = x^5 \coth(x) \)
    - \( u_4(x) = x^6 \coth(x) \)
    - \( u_5(x) = x^7 \coth(x) \)
    - \( u_6(x) = x^8 \coth(x) \)
    - \( u_7(x) = x^9 \coth(x) \)
    - \( u_8(x) = x^{10} \coth(x) \)
    - \( u_9(x) = x^{11} \coth(x) \)
    - \( u_{10}(x) = x^{12} \coth(x) \)

11. For \( v(x) = x^5 \cos^2(x) \):
    - \( v_1(x) = x^5 \cos^2(x) \)
    - \( v_2(x) = x^6 \cos^2(x) \)
    - \( v_3(x) = x^7 \cos^2(x) \)
    - \( v_4(x) = x^8 \cos^2(x) \)
    - \( v_5(x) = x^9 \cos^2(x) \)
    - \( v_6(x) = x^{10} \cos^2(x) \)
    - \( v_7(x) = x^{11} \cos^2(x) \)
    - \( v_8(x) = x^{12} \cos^2(x) \)
    - \( v_9(x) = x^{13} \cos^2(x) \)
    - \( v_{10}(x) = x^{14} \cos^2(x) \)

12. For \( w(x) = x^2 \sin^3(x) \):
    - \( w_1(x) = x^2 \sin^3(x) \)
    - \( w_2(x) = x^3 \sin^3(x) \)
    - \( w_3(x) = x^4 \sin^3(x) \)
    - \( w_4(x) = x^5 \sin^3(x) \)
    - \( w_5(x) = x^6 \sin^3(x) \)
    - \( w_6(x) = x^7 \sin^3(x) \)
    - \( w_7(x) = x^8 \sin^3(x) \)
    - \( w_8(x) = x^9 \sin^3(x) \)
    - \( w_9(x) = x^{10} \sin^3(x) \)
    - \( w_{10}(x) = x^{11} \sin^3(x) \)

13. For \( z(x) = x^3 \arcsin(x) \):
    - \( z_1(x) = x^3 \arcsin(x) \)
    - \( z_2(x) = x^4 \arcsin(x) \)
    - \( z_3(x) = x^5 \arcsin(x) \)
    - \( z_4(x) = x^6 \arcsin(x) \)
    - \( z_5(x) = x^7 \arcsin(x) \)
    - \( z_6(x) = x^8 \arcsin(x) \)
    - \( z_7(x) = x^9 \arcsin(x) \)
    - \( z_8(x) = x^{10} \arcsin(x) \)
    - \( z_9(x) = x^{11} \arcsin(x) \)
    - \( z_{10}(x) = x^{12} \arcsin(x) \)

14. For \( b(x) = x^4 \arcsin(x) \):
    - \( b_1(x) = x^4 \arcsin(x) \)
    - \( b_2(x) = x^5 \arcsin(x) \)
    - \( b_3(x) = x^6 \arcsin(x) \)
    - \( b_4(x) = x^7 \arcsin(x) \)
    - \( b_5(x) = x^8 \arcsin(x) \)
    - \( b_6(x) = x^9 \arcsin(x) \)
    - \( b_7(x) = x^{10} \arcsin(x) \)
    - \( b_8(x) = x^{11} \arcsin(x) \)
    - \( b_9(x) = x^{12} \arcsin(x) \)
    - \( b_{10}(x) = x^{13} \arcsin(x) \)

15. For \( a(x) = x^3 \log(\sin(x)) \):
    - \( a_1(x) = x^3 \log(\sin(x)) \)
    - \( a_2(x) = x^4 \log(\sin(x)) \)
    - \( a_3(x) = x^5 \log(\sin(x)) \)
    - \( a_4(x) = x^6 \log(\sin(x)) \)
    - \( a_5(x) = x^7 \log(\sin(x)) \)
    - \( a_6(x) = x^8 \log(\sin(x)) \)
    - \( a_7(x) = x^9 \log(\sin(x)) \)
    - \( a_8(x) = x^{10} \log(\sin(x)) \)
    - \( a_9(x) = x^{11} \log(\sin(x)) \)
    - \( a_{10}(x) = x^{12} \log(\sin(x)) \)
